@prefix rdf: <http://www.w3.org/1999/02/22-rdf-syntax-ns#> .
@prefix rdfs: <http://www.w3.org/2000/01/rdf-schema#> .
@prefix xsd: <http://www.w3.org/2001/XMLSchema#> .
@prefix xml: <http://www.w3.org/XML/1998/namespace> .
@prefix dc: <http://purl.org/dc/elements/1.1/#> .
@prefix owl: <http://www.w3.org/2002/07/owl#> .
@prefix owl2: <http://www.w3.org/2006/12/owl2#> .
@prefix swrlx: <http://www.w3.org/2003/11/swrlx#> .
@prefix event: <http://purl.org/NET/c4dm/event.owl#> .
@prefix time: <http://www.w3.org/2006/time#> .
@prefix foaf: <http://xmlns.com/foaf/0.1/> .
@prefix tapio: <https://github.com/Rburkett/icas-ontology/edit/master/ontology/tapio#> .
@prefix user: <https://github.com/Rburkett/icas-ontology/edit/master/ontology/user#> .
@prefix host: <https://github.com/Rburkett/icas-ontology/edit/master/ontology/host#> .
@prefix process: <https://github.com/Rburkett/icas-ontology/edit/master/ontology/process#> .
@prefix ipnet: <https://github.com/Rburkett/icas-ontology/edit/master/ontology/ipnet#> .
@prefix : <https://github.com/Rburkett/icas-ontology/edit/master/ontology/authentication#> .

<https://github.com/Rburkett/icas-ontology/edit/master/ontology/authentication>
    dc:creator "Invincea Labs"@en ;
    dc:date "2014" ;
    dc:description "Describes elements related to authentication mechanisms in systems that grant identity to users and requests to map them to privileges"@en ;
    a owl:Ontology ;
    rdfs:comment "Describes elements related to authentication mechanisms in systems that grant identity to users and requests to map them to privileges"@en ;
    rdfs:label "Authentication Ontology"@en ;
    owl:imports <https://github.com/Rburkett/icas-ontology/edit/master/ontology/host>, <https://github.com/Rburkett/icas-ontology/edit/master/ontology/user> ;
    owl:versionInfo "1.0" .

:ActiveDirectory
    a :AuthProvider, owl:NamedIndividual ;
    rdfs:comment "An ActiveDirectory authentication service." ;
    rdfs:label "LDAP Service"@en .

:AuthEvent
    a owl:Class ;
    rdfs:comment "A generic attempt by a user to authenticate to a service."@en ;
    rdfs:label "Authentication Event"@en ;
    rdfs:subClassOf event:Event .

:AuthProvider
    a owl:Class ;
    rdfs:comment "A provider capable of providing authentication services. Examples might include RADIUS, local, etc."@en ;
    rdfs:label "Authentication Provider"@en ;
    rdfs:subClassOf owl:Thing .

:Credential
    a owl:Class ;
    rdfs:comment "A credential that can be used for authentication."@en ;
    rdfs:label "Credential"@en ;
    rdfs:subClassOf owl:Thing .

:LDAP
    a :AuthProvider, owl:NamedIndividual ;
    rdfs:comment "An LDAP authentication service." ;
    rdfs:label "LDAP Authenticator"@en .

:LocalAccount
    a :AuthProvider, owl:NamedIndividual ;
    rdfs:comment "A local host account, such as controlled by PAM or Windows Account Services."@en ;
    rdfs:label "Local Host Account Authenticator"@en .

:LoginCredential
    a owl:Class ;
    rdfs:comment "The generic set of credentials which are authenticated using a username  and (optionally) a password."@en ;
    rdfs:label "Login Credential"@en ;
    rdfs:subClassOf :Credential .

:RADIUS
    a :AuthProvider, owl:NamedIndividual ;
    rdfs:comment "A RADIUS remote authentication service." ;
    rdfs:label "RADIUS Authenticator"@en .

:authBy
    a owl:FunctionalProperty, owl:ObjectProperty ;
    rdfs:comment "Relates an authentication provider to an authentication event. "@en ;
    rdfs:domain :AuthEvent ;
    rdfs:label "authenticated By"@en ;
    rdfs:range :AuthProvider ;
    rdfs:subPropertyOf event:agent .

:authRequestedFrom
    a owl:FunctionalProperty, owl:ObjectProperty ;
    rdfs:comment "The Source of the authentication attempt. The client endpoint of an authentication connection."@en ;
    rdfs:domain :AuthEvent ;
    rdfs:label "authentication attempted from" ;
    rdfs:range host:Host, ipnet:Address ;
    rdfs:subPropertyOf event:factor .

:authStatus
    a owl:DatatypeProperty, owl:FunctionalProperty ;
    rdfs:comment "The status of an authentication event. Could be 'success', 'failure', 'inprogress', etc."@en ;
    rdfs:domain :AuthEvent ;
    rdfs:label "Authentication Status"@en ;
    rdfs:range xsd:string .

:authToHost
    a owl:FunctionalProperty, owl:ObjectProperty ;
    rdfs:comment "The host that this authentication event is providing authentication for."@en ;
    rdfs:domain :AuthEvent ;
    rdfs:label "authenticating To" ;
    rdfs:range host:Host ;
    rdfs:subPropertyOf event:factor .

:authenticatesAgainstRealm
    a owl:FunctionalProperty, owl:ObjectProperty ;
    rdfs:domain :AuthProvider ;
    rdfs:label "authenticates against account realm"@en ;
    rdfs:range user:Realm .

:hasCredential
    a owl:ObjectProperty ;
    rdfs:comment "Links user#UserAccount to credential sets."@en ;
    rdfs:domain user:UserAccount ;
    rdfs:label "has credential"@en ;
    rdfs:range :Credential ;
    owl:equivalentProperty user:hasCredential .

:loginName
    tapio:signaturePriority 2 ;
    a owl:DatatypeProperty, owl:FunctionalProperty ;
    rdfs:comment "The specific string used to identify an account via keyboard input"@en ;
    rdfs:domain :LoginCredential ;
    rdfs:label "Login Name"@en ;
    rdfs:range xsd:string .

:loginPass
    a owl:DatatypeProperty, owl:FunctionalProperty ;
    rdfs:comment "A password or passphrase used for login credentials"@en ;
    rdfs:domain :LoginCredential ;
    rdfs:label "Login Password"@en ;
    rdfs:range xsd:string .

:sessionId
    tapio:signaturePriority 1 ;
    a owl:DatatypeProperty, owl:FunctionalProperty ;
    rdfs:comment "The unique session ID given to this authentication event."@en ;
    rdfs:domain :AuthEvent ;
    rdfs:label "Unique ID for the authentication session"@en ;
    rdfs:range xsd:string .

:usingCredential
    a owl:FunctionalProperty, owl:ObjectProperty ;
    rdfs:comment "The credential token presented to verify  that the user is who they attest to be during this authentication session"@en ;
    rdfs:domain :AuthEvent ;
    rdfs:label "Authenticated With Credential"@en ;
    rdfs:range :Credential ;
    rdfs:subPropertyOf event:factor .

