@prefix rdf: <http://www.w3.org/1999/02/22-rdf-syntax-ns#> .
@prefix rdfs: <http://www.w3.org/2000/01/rdf-schema#> .
@prefix xsd: <http://www.w3.org/2001/XMLSchema#> .
@prefix xml: <http://www.w3.org/XML/1998/namespace> .
@prefix dc: <http://purl.org/dc/elements/1.1/#> .
@prefix owl: <http://www.w3.org/2002/07/owl#> .
@prefix owl2: <http://www.w3.org/2006/12/owl2#> .
@prefix swrl: <http://www.w3.org/2003/11/swrl#> .
@prefix swrlx: <http://www.w3.org/2003/11/swrlx#> .
@prefix swrlb: <http://www.w3.org/2003/11/swrlb#> .
@prefix event: <http://purl.org/NET/c4dm/event.owl#> .
@prefix time: <http://www.w3.org/2006/time#> .
@prefix foaf: <http://xmlns.com/foaf/0.1/> .
@prefix mere: <http://www.bbn.com/ontologies/domain/foundation/mereology#> .
@prefix tapio: <https://github.com/Rburkett/icas-ontology/edit/master/ontology/tapio#> .
@prefix ipnet: <https://github.com/Rburkett/icas-ontology/edit/master/ontology/ipnet#> .
@prefix host: <https://github.com/Rburkett/icas-ontology/edit/master/ontology/host#> .
@prefix software: <https://github.com/Rburkett/icas-ontology/edit/master/ontology/software#> .
@prefix : <https://github.com/Rburkett/icas-ontology/edit/master/ontology/controls#> .

<https://github.com/Rburkett/icas-ontology/edit/master/ontology/controls>
    dc:creator "Invincea Labs"@en ;
    dc:date "2014" ;
    dc:description "an ontology describing Security controls and their outputs"@en ;
    a owl:Ontology ;
    rdfs:comment "an ontology describing Security controls and their outputs."@en ;
    rdfs:label "Security Controls ontology"@en ;
    owl:versionInfo "1.0" .

:Action
    a owl:Class ;
    rdfs:comment "Alerts are responses from a security control that only inform that a condition described in a rule has been detected"@en ;
    rdfs:label "Action"@en ;
    rdfs:subClassOf :Response .

:Alert
    a owl:Class ;
    rdfs:comment "Alerts are responses from a security control that only inform that a condition described in a rule has been detected"@en ;
    rdfs:label "Alert" ;
    rdfs:subClassOf :Response .

:CorrectiveSecurityControl
    a owl:Class ;
    rdfs:comment "Corrective Security controls take action (and usually also generate alerts) upon detection of matching conditions"@en ;
    rdfs:label "Corrective Security Control"@en ;
    rdfs:subClassOf :SecurityControl .

:DetectiveSecurityControl
    a owl:Class ;
    rdfs:comment "Detective Security controls generate alerts upon detection of matching conditions"@en ;
    rdfs:label "Detective Security Control"@en ;
    rdfs:subClassOf :SecurityControl .

:Policy
    a owl:Class ;
    rdfs:comment "Policies, in the context of security controls, are grouping objects containing rules, that enforce or detect deviations from a stated organizational policy"@en ;
    rdfs:label "Policy"@en ;
    rdfs:subClassOf mere:SimpleComposite, owl:Thing .

:PreventativeSecurityControl
    a owl:Class ;
    rdfs:label "Preventative Security Control"@en ;
    rdfs:subClassOf :SecurityControl .

:Response
    a owl:Class ;
    rdfs:comment "Controls generate Responses according to rule sets - these responses may be passive (alerting) or active (actions)."@en ;
    rdfs:label "Response"@en ;
    rdfs:subClassOf event:Event .

:Rule
    a owl:Class ;
    rdfs:comment "Security controls produce responses according to conditions described in rules, usually with each rule producing a uniquely-named response"@en ;
    rdfs:label "Rule"@en ;
    rdfs:subClassOf mere:Atom, owl:Thing .

:SecurityControl
    a owl:Class, foaf:Agent ;
    rdfs:comment "A technical security control, embodied as active software monitoring the activity of one or more hosts or networks."@en ;
    rdfs:label "Security Control"@en ;
    rdfs:subClassOf owl:Thing .

:enforcesPolicy
    a owl:ObjectProperty ;
    rdfs:domain :SecurityControl ;
    rdfs:label "This control is configured with rules described in the following policy group"@en, "enforces policy"@en ;
    rdfs:range :Policy .

:generatedBy
    tapio:signaturePriority 1 ;
    a owl:ObjectProperty ;
    rdfs:comment "this response was generated by this security control"@en ;
    rdfs:domain :Response ;
    rdfs:label "was generated by"@en ;
    rdfs:range :SecurityControl ;
    rdfs:subPropertyOf event:agent ;
    owl:inverseOf :generatedResponse .

:generatedResponse
    a owl:InverseFunctionalProperty, owl:ObjectProperty ;
    rdfs:comment "this control generated the following action in response to a rule in its configuration"@en ;
    rdfs:domain :SecurityControl ;
    rdfs:label "generated action"@en ;
    rdfs:range :Action, :Alert ;
    rdfs:subPropertyOf event:agent_in ;
    owl:inverseOf :generatedBy .

:hasRule
    a owl:ObjectProperty ;
    rdfs:comment "Policies contain individual rules that describe the conditions that deviate from (or enforce) the goals of the policy"@en ;
    rdfs:domain :Policy ;
    rdfs:label "has rule"@en ;
    rdfs:range :Rule ;
    rdfs:subPropertyOf mere:hasPart ;
    owl:inverseOf :inPolicy .

:hasSource
    a owl:FunctionalProperty, owl:ObjectProperty ;
    rdfs:comment "this alert was generated as a result of the actions of this source"@en ;
    rdfs:domain :Alert ;
    rdfs:label "has source"@en ;
    rdfs:range owl:Thing ;
    rdfs:subPropertyOf event:factor .

:hasTarget
    a owl:ObjectProperty ;
    rdfs:comment "this response action was applied to this target "@en ;
    rdfs:domain :Action ;
    rdfs:label "has target"@en ;
    rdfs:range owl:Thing ;
    rdfs:subPropertyOf event:factor .

:inPolicy
    a owl:ObjectProperty ;
    rdfs:comment "Policies contain individual rules that describe the conditions that deviate from (or enforce) the goals of the policy"@en ;
    rdfs:domain :Rule ;
    rdfs:label "has rule"@en ;
    rdfs:range :Policy ;
    rdfs:subPropertyOf mere:partOf ;
    owl:inverseOf :hasRule .

:monitorsHost
    a owl:ObjectProperty ;
    rdfs:comment "this security control has visibility and governance over the following host"@en ;
    rdfs:domain :SecurityControl ;
    rdfs:label "monitors host"@en ;
    rdfs:range host:Host .

:monitorsSubnet
    a owl:ObjectProperty ;
    rdfs:comment "this security control has visibility and governance over the following subnet"@en ;
    rdfs:domain :SecurityControl ;
    rdfs:label "monitors subnet"@en ;
    rdfs:range ipnet:SubNet .

:ruleID
    a owl:DatatypeProperty, owl:FunctionalProperty ;
    rdfs:comment "Controls typically have rule sets that govern how and what they respond to. This field is used to identify the particular rule this response was generated via, using the identity native to the source control"@en ;
    rdfs:domain :Rule ;
    rdfs:label "Rule ID"@en ;
    rdfs:range xsd:normalizedString ;
    rdfs:subPropertyOf event:literal_factor .

:runsOnHost
    a owl:FunctionalProperty, owl:ObjectProperty ;
    rdfs:domain :SecurityControl ;
    rdfs:label "The host that this security control operates from"@en, "runs on host"@en ;
    rdfs:range host:Host .

:triggeredByRule
    a owl:FunctionalProperty, owl:ObjectProperty ;
    rdfs:comment "this response was triggered by conditions by conditions described in this rule"@en ;
    rdfs:domain :Response ;
    rdfs:label "was triggered by rule"@en ;
    rdfs:range :Rule ;
    rdfs:subClassOf event:factor ;
    owl:inverseOf :triggeredResponse .

:triggeredResponse
    a owl:InverseFunctionalProperty, owl:ObjectProperty ;
    rdfs:comment "this rule defines the matching conditions that caused the security control to create this response"@en ;
    rdfs:domain :Rule ;
    rdfs:label "triggered response"@en ;
    rdfs:range :Response ;
    rdfs:subClassOf event:factor_in ;
    owl:inverseOf :triggeredByRule .

