@prefix rdf: <http://www.w3.org/1999/02/22-rdf-syntax-ns#> .
@prefix rdfs: <http://www.w3.org/2000/01/rdf-schema#> .
@prefix xsd: <http://www.w3.org/2001/XMLSchema#> .
@prefix xml: <http://www.w3.org/XML/1998/namespace> .
@prefix dc: <http://purl.org/dc/elements/1.1/#> .
@prefix owl: <http://www.w3.org/2002/07/owl#> .
@prefix owl2: <http://www.w3.org/2006/12/owl2#> .
@prefix swrlx: <http://www.w3.org/2003/11/swrlx#> .
@prefix event: <http://purl.org/NET/c4dm/event.owl#> .
@prefix time: <http://www.w3.org/2006/time#> .
@prefix foaf: <http://xmlns.com/foaf/0.1/> .
@prefix mere: <http://www.bbn.com/ontologies/domain/foundation/mereology#> .
@prefix nic: <https://github.com/Rburkett/icas-ontology/edit/master/ontology/nic#> .
@prefix oui: <https://github.com/Rburkett/icas-ontology/edit/master/ontology/oui#> .
@prefix log: <https://github.com/Rburkett/icas-ontology/edit/master/ontology/log#> .
@prefix user: <https://github.com/Rburkett/icas-ontology/edit/master/ontology/user#> .
@prefix filesystem: <https://github.com/Rburkett/icas-ontology/edit/master/ontology/filesystem#> .
@prefix tapio: <https://github.com/Rburkett/icas-ontology/edit/master/ontology/tapio#> .
@prefix ipnet: <https://github.com/Rburkett/icas-ontology/edit/master/ontology/ipnet#> .
@prefix hardware: <https://github.com/Rburkett/icas-ontology/edit/master/ontology/hardware#> .
@prefix mime: <https://github.com/Rburkett/icas-ontology/edit/master/ontology/mime#> .
@prefix process: <https://github.com/Rburkett/icas-ontology/edit/master/ontology/process#> .
@prefix host: <https://github.com/Rburkett/icas-ontology/edit/master/ontology/host#> .
@prefix : <https://github.com/Rburkett/icas-ontology/edit/master/ontology/memory#> .

<https://github.com/Rburkett/icas-ontology/edit/master/ontology/memory>
    dc:creator "Invincea Labs"@en ;
    dc:date "2014" ;
    dc:description "Describes high level organization and addressing of objects within Random Access Memory"@en ;
    a owl:Ontology ;
    rdfs:comment "Describes high level organization and addressing of objects within Random Access Memory"@en ;
    rdfs:label "An ontology for mapping regions of Memory Objects into their functional purposes."@en ;
    owl:imports <https://github.com/Rburkett/icas-ontology/edit/master/ontology/filesystem>, <https://github.com/Rburkett/icas-ontology/edit/master/ontology/process> ;
    owl:versionInfo "1.0" .

:Code
    a owl:Class ;
    rdfs:comment "An area of system memory assigned for executable code"@en ;
    rdfs:label "Region of Memory"@en ;
    rdfs:subClassOf :MemoryBlock .

:Data
    a owl:Class ;
    rdfs:comment "An area of system memory assigned for non-executable data"@en ;
    rdfs:label "Data Region of Memory"@en ;
    rdfs:subClassOf :MemoryBlock .

:MemoryAddressPhy32
    a rdfs:Datatype ;
    rdfs:comment "A 32bit address, relative to the host system's entire memory space"@en ;
    rdfs:label "32-Bit Physical Memory Address"@en ;
    owl:equivalentClass xsd:unsignedInt .

:MemoryAddressPhy64
    a rdfs:Datatype ;
    rdfs:comment "A 64bit address, relative to the host system's entire memory space"@en ;
    rdfs:label "64-Bit Physical Memory Address"@en ;
    owl:equivalentClass xsd:unsignedInt .

:MemoryAddressVirt32
    a rdfs:Datatype ;
    rdfs:comment "A 32bit address, relative to the host system's entire memory space"@en ;
    rdfs:label "32-Bit Virtual Memory Address"@en ;
    owl:equivalentClass xsd:unsignedInt .

:MemoryAddressVirt64
    a rdfs:Datatype ;
    rdfs:comment "A 64bit address, relative to the host system's entire memory space"@en ;
    rdfs:label "64-Bit Virtual Memory Address"@en ;
    owl:equivalentClass xsd:unsignedLong .

:MemoryBlock
    a owl:Class ;
    rdfs:comment "An area of system memory, contiguous between a start and end address"@en ;
    rdfs:label "Region of Memory"@en ;
    rdfs:subClassOf mere:Composite, owl:Thing .

:MetaCode
    a owl:Class ;
    rdfs:comment "An area of system memory assigned for execution-tracking items, such as the Heap and Stack"@en ;
    rdfs:label "MetaCode Region of Memory"@en ;
    rdfs:subClassOf :Code .

:MetaData
    a owl:Class ;
    rdfs:comment "An area of system memory assigned for data-tracking items, such as item index pointers"@en ;
    rdfs:label "MetaData Region of Memory"@en ;
    rdfs:subClassOf :Data .

:beginsAtAddress
    tapio:signaturePriority 1 ;
    a owl:DatatypeProperty, owl:FunctionalProperty ;
    rdfs:domain :MemoryBlock ;
    rdfs:label "Begins at Address"@en ;
    rdfs:range :MemoryAddressPhy32, :MemoryAddressPhy64, :MemoryAddressVirt32, :MemoryAddressVirt64 .

:endsAtAddress
    tapio:signaturePriority 2 ;
    a owl:DatatypeProperty, owl:FunctionalProperty ;
    rdfs:domain :MemoryBlock ;
    rdfs:label "Ends at Address"@en ;
    rdfs:range :MemoryAddressPhy32, :MemoryAddressPhy64, :MemoryAddressVirt32, :MemoryAddressVirt64 .

:hasMemoryBlock
    a owl:ObjectProperty ;
    rdfs:comment "This process owns the identified block of memory"@en ;
    rdfs:domain process:Process ;
    rdfs:label "contains memory region"@en ;
    rdfs:range :MemoryBlock ;
    owl:inverseOf :isOwnedByProcess .

:hasSize
    a owl:DatatypeProperty, owl:FunctionalProperty ;
    rdfs:domain :MemoryBlock ;
    rdfs:label "Has total size"@en ;
    rdfs:range xsd:positiveInteger .

:isOwnedByProcess
    a owl:FunctionalProperty, owl:ObjectProperty ;
    rdfs:comment "the executing process that owns this region of memory"@en ;
    rdfs:domain :MemoryBlock ;
    rdfs:label "is owned by process"@en ;
    rdfs:range process:Process ;
    owl:inverseOf :hasMemoryBlock .

:mappedFromFile
    a owl:FunctionalProperty, owl:ObjectProperty ;
    rdfs:comment "the contents of this memory block were drawn from this file."@en ;
    rdfs:domain :MemoryBlock ;
    rdfs:label "is loaded from contents of file"@en ;
    rdfs:range filesystem:File .

:sharesVirtualMemorySpace
    a owl:ObjectProperty, owl:SymmetricProperty ;
    rdfs:domain :MemoryBlock ;
    rdfs:label "shares virtual memory space with"@en ;
    rdfs:range :MemoryBlock .

