@prefix rdf: <http://www.w3.org/1999/02/22-rdf-syntax-ns#> .
@prefix rdfs: <http://www.w3.org/2000/01/rdf-schema#> .
@prefix xsd: <http://www.w3.org/2001/XMLSchema#> .
@prefix xml: <http://www.w3.org/XML/1998/namespace> .
@prefix dc: <http://purl.org/dc/elements/1.1/#> .
@prefix owl: <http://www.w3.org/2002/07/owl#> .
@prefix owl2: <http://www.w3.org/2006/12/owl2#> .
@prefix swrlx: <http://www.w3.org/2003/11/swrlx#> .
@prefix event: <http://purl.org/NET/c4dm/event.owl#> .
@prefix time: <http://www.w3.org/2006/time#> .
@prefix foaf: <http://xmlns.com/foaf/0.1/> .
@prefix tapio: <https://github.com/Rburkett/icas-ontology/edit/master/ontology/tapio#> .
@prefix nic: <https://github.com/Rburkett/icas-ontology/edit/master/ontology/nic#> .
@prefix : <https://github.com/Rburkett/icas-ontology/edit/master/ontology/oui#> .

<https://github.com/Rburkett/icas-ontology/edit/master/ontology/oui>
    dc:creator "Invincea Labs"@en ;
    dc:date "2014" ;
    dc:description "Describes OUI numbers that match hardware interfaces to their manufacturer."@en ;
    a owl:Ontology ;
    rdfs:comment "Describes OUI numbers that match hardware interfaces to their manufacturer."@en ;
    rdfs:label "Organizationally Unique Identifier Ontology"@en ;
    owl:versionInfo "1.0" .

:OUI
    a owl:Class ;
    rdfs:comment "OUI's are used to identify the manufacturer of network equipment via the physical address they present to the network, and assist that addressing collisions do not occur between manufacturers"@en ;
    rdfs:label "Organizationally Unique Identifier"@en ;
    rdfs:subClassOf owl:Thing .

:OUId
    a owl:DatatypeProperty, owl:FunctionalProperty ;
    rdfs:domain :OUI ;
    rdfs:label "OUI Value"@en ;
    rdfs:range xsd:hexBinary .

:Vendor
    a owl:Class ;
    rdfs:label "Vendor"@en ;
    rdfs:subClassOf owl:Thing .

:issuedToVendor
    a owl:FunctionalProperty, owl:ObjectProperty ;
    rdfs:comment "the organization this OID is registered with to serialize their products with."@en ;
    rdfs:domain :OUI ;
    rdfs:label "is registered with"@en ;
    rdfs:range :Vendor ;
    owl:inverseOf :ownsOUI .

:ownsOUI
    a owl:InverseFunctionalProperty, owl:ObjectProperty ;
    rdfs:domain :Vendor ;
    rdfs:label "owns the following OUI"@en ;
    rdfs:range :OUI ;
    owl:inverseOf :issuedToVendor .

