@prefix rdf: <http://www.w3.org/1999/02/22-rdf-syntax-ns#> .
@prefix owl: <http://www.w3.org/2002/07/owl#> .
@prefix time: <http://www.w3.org/2006/time#> .
@prefix rdfs: <http://www.w3.org/2000/01/rdf-schema#> .
@prefix vs: <http://www.w3.org/2003/06/sw-vocab-status/ns#> .
@prefix foaf: <http://xmlns.com/foaf/0.1/> .
@prefix geo: <http://www.w3.org/2003/01/geo/wgs84_pos#> .
@prefix dc: <http://purl.org/dc/elements/1.1/> .
@prefix mere: <http://www.bbn.com/ontologies/domain/foundation/mereology#> .
@prefix xsd: <http://www.w3.org/2001/XMLSchema#> .
@prefix tapio: <https://github.com/Rburkett/icas-ontology/edit/master/ontology/tapio#> .
@prefix : <http://purl.org/NET/c4dm/event.owl#> .

<http://purl.org/NET/c4dm/event.owl>
    dc:date "$Date: 2007/06/29 15:25:11 $"@en ;
    dc:description """
			This ontology deals with the notion of reified events---
			events seen as first-class objects. It only defines one
			concept: Event, which may have agents (actively
			participating), factors (passively participating), products,
			and a location in space and time. 

			Regarding the ontological status of event tokens, they are seen
			as the way cognitive agents classify space/time regions
			"""@en ;
    dc:title "The Event ontology"@en ;
    a owl:Ontology, owl:Thing ;
    rdfs:label "The Event ontology"@en ;
    owl:imports <http://www.w3.org/2006/time> ;
    owl:versionInfo "Revision: 1.01"@en ;
    foaf:maker <http://moustaki.org/foaf.rdf#moustaki> .

:Event
    a owl:Class ;
    rdfs:comment """
				An arbitrary classification of a space/time region, by a 
				cognitive agent. An event may have actively participating agents,
				passive factors, products, and a location in space/time.
				"""@en ;
    rdfs:label "Event"@en ;
    rdfs:subClassOf mere:Composite ;
    vs:term_status "stable"@en .

:Factor
    a owl:Class ;
    rdfs:comment "Everything used as a factor in an event"@en ;
    rdfs:label "Factor"@en ;
    owl:disjointWith foaf:Agent ;
    owl:equivalentClass [
        a owl:Restriction ;
        owl:onProperty :factor_of ;
        owl:someValuesFrom :Event
    ] ;
    vs:term_status "stable"@en .

:Product
    a owl:Class ;
    rdfs:comment "Everything produced by an event"@en ;
    rdfs:label "Product"@en ;
    owl:equivalentClass [
        a owl:Restriction ;
        owl:onProperty :produced_in ;
        owl:someValuesFrom :Event
    ] ;
    vs:term_status "stable"@en .

:agent
    tapio:signaturePriority 1 ;
    a owl:ObjectProperty ;
    rdfs:comment "Relates an event to an active agent (a person, a computer, ... :-) )"@en ;
    rdfs:domain :Event ;
    rdfs:label "agent"@en ;
    rdfs:range foaf:Agent ;
    owl:equivalentProperty :hasAgent ;
    owl:inverseOf :agent_in ;
    vs:term_status "stable"@en .

:agent_in
    a owl:ObjectProperty ;
    vs:term_status "stable"@en .

:factor
    a owl:ObjectProperty ;
    rdfs:comment "Relates an event to a passive factor (a tool, an instrument, an abstract cause...)"@en ;
    rdfs:domain :Event ;
    rdfs:label "factor"@en ;
    owl:equivalentProperty :hasFactor ;
    owl:inverseOf :factor_of ;
    vs:term_status "stable"@en .

:factor_of
    a owl:ObjectProperty ;
    vs:term_status "stable"@en .

:literal_factor
    a owl:DatatypeProperty ;
    rdfs:comment """
				Relates an event to a factor which can be described as a literal. This property
				should not be used as-is, but should be subsumed by other, more specific, properties
				(like an hypothetic :weatherCelsius, linking an event to a temperature).
				"""@en ;
    rdfs:domain :Event ;
    rdfs:label "literal factor"@en ;
    owl:equivalentProperty :hasLiteralFactor ;
    vs:term_status "stable"@en .

:place
    a owl:ObjectProperty ;
    rdfs:comment "Relates an event to a spatial object."@en ;
    rdfs:domain :Event ;
    rdfs:label "place"@en ;
    rdfs:range geo:SpatialThing ;
    vs:term_status "stable"@en .

:produced_in
    a owl:ObjectProperty ;
    vs:term_status "stable"@en .

:product
    a owl:ObjectProperty ;
    rdfs:comment "Relates an event to something produced during the event---a sound, a pie, whatever..."@en ;
    rdfs:domain :Event ;
    rdfs:label "product"@en ;
    owl:equivalentProperty :hasProduct ;
    owl:inverseOf :produced_in ;
    vs:term_status "stable"@en .

:sub_event
    a owl:ObjectProperty ;
    rdfs:comment "This property provides a way to split a complex event (for example, a performance involving several musicians) into simpler ones (one event per musician)."@en ;
    rdfs:domain :Event ;
    rdfs:label "sub-event"@en ;
    rdfs:range :Event ;
    rdfs:subPropertyOf mere:directlyHasPart ;
    owl:equivalentProperty :hasSubEvent ;
    vs:term_status "stable"@en .

:time
    tapio:signaturePriority 2 ;
    a owl:ObjectProperty ;
    rdfs:comment """
				Relates an event to a time object, classifying a time region (either instantaneous or having an extent).
				By using the Timeline ontology here, you can define event happening on a recorded track or on any 
				media with a temporal extent.
				"""@en ;
    rdfs:domain :Event ;
    rdfs:label "time"@en ;
    rdfs:range time:TemporalEntity ;
    vs:term_status "stable"@en .

