@prefix rdf: <http://www.w3.org/1999/02/22-rdf-syntax-ns#> .
@prefix rdfs: <http://www.w3.org/2000/01/rdf-schema#> .
@prefix xsd: <http://www.w3.org/2001/XMLSchema#> .
@prefix xml: <http://www.w3.org/XML/1998/namespace> .
@prefix dc: <http://purl.org/dc/elements/1.1/#> .
@prefix owl: <http://www.w3.org/2002/07/owl#> .
@prefix owl2: <http://www.w3.org/2006/12/owl2#> .
@prefix swrlx: <http://www.w3.org/2003/11/swrlx#> .
@prefix event: <http://purl.org/NET/c4dm/event.owl#> .
@prefix time: <http://www.w3.org/2006/time#> .
@prefix foaf: <http://xmlns.com/foaf/0.1/> .
@prefix mere: <http://www.bbn.com/ontologies/domain/foundation/mereology#> .
@prefix tapio: <https://github.com/Rburkett/icas-ontology/edit/master/ontology/tapio#> .
@prefix host: <https://github.com/Rburkett/icas-ontology/edit/master/ontology/host#> .
@prefix ipnet: <https://github.com/Rburkett/icas-ontology/edit/master/ontology/ipnet#> .
@prefix process: <https://github.com/Rburkett/icas-ontology/edit/master/ontology/process#> .
@prefix software: <https://github.com/Rburkett/icas-ontology/edit/master/ontology/software#> .
@prefix filesystem: <https://github.com/Rburkett/icas-ontology/edit/master/ontology/filesystem#> .
@prefix controls: <https://github.com/Rburkett/icas-ontology/edit/master/ontology/controls#> .
@prefix authentication: <https://github.com/Rburkett/icas-ontology/edit/master/ontology/authentication#> .
@prefix user: <https://github.com/Rburkett/icas-ontology/edit/master/ontology/user#> .
@prefix uri: <https://github.com/Rburkett/icas-ontology/edit/master/ontology/uri#> .
@prefix : <https://github.com/Rburkett/icas-ontology/edit/master/ontology/log#> .

<https://github.com/Rburkett/icas-ontology/edit/master/ontology/log>
    dc:creator "Invincea Labs"@en ;
    dc:date "2014" ;
    dc:description "describes point-in-time events from software"@en ;
    a owl:Ontology ;
    rdfs:comment "describes point-in-time events from software"@en ;
    rdfs:label "Log and Events Ontology"@en ;
    owl:versionInfo "1.0" .

:AccessDenied
    a owl:Class ;
    rdfs:comment "The access request was denied - the requesting identity is not authorized to use this service or resource"@en ;
    rdfs:label "Access Denied Event"@en ;
    rdfs:subClassOf :AccessResponse .

:AccessFailed
    a owl:Class ;
    rdfs:comment "The access request failed - the requested resource or service is not available"@en ;
    rdfs:label "Access Failed Event"@en ;
    rdfs:subClassOf :AccessResponse .

:AccessRequest
    a owl:Class ;
    rdfs:comment "This log entry describes a request for access to a resource."@en ;
    rdfs:label "Access Request Event"@en ;
    rdfs:subClassOf :Request .

:AccessResponse
    a owl:Class ;
    rdfs:comment "This is a response to a request for access - usually in response to a request for particular content or service"@en ;
    rdfs:label "Access Response Event"@en ;
    rdfs:subClassOf :Response .

:AccessSuccessful
    a owl:Class ;
    rdfs:comment "The access request was succesful - the requested resource or service has been delivered to the requester"@en ;
    rdfs:label "Successful Access Event"@en ;
    rdfs:subClassOf :AccessResponse .

:AuthenticationDenied
    a owl:Class ;
    rdfs:comment "The authentication request was specifically denied - typically because of incorrect credentials in the request"@en ;
    rdfs:label "Authentication Denied Event"@en ;
    rdfs:subClassOf :AuthenticationResponse .

:AuthenticationFailed
    a owl:Class ;
    rdfs:comment "The authentication request failed to process - typically because of an error in the authentication mechanism"@en ;
    rdfs:label "Authentication Failed Event"@en ;
    rdfs:subClassOf :AuthenticationResponse .

:AuthenticationRequest
    a owl:Class ;
    rdfs:comment "This log entry describes a request to uniquely identify the source, usually via credentials"@en ;
    rdfs:label "Authentication Request Event"@en ;
    rdfs:subClassOf :Request .

:AuthenticationResponse
    a owl:Class ;
    rdfs:comment "This is a response to a request for Authentication - typically in response to credentials presented during that request"@en ;
    rdfs:label "Authentication Response Event"@en ;
    rdfs:subClassOf :Response .

:AuthorizationDenied
    a owl:Class ;
    rdfs:comment "The authorization request was Denied - the requesting identity is not authorized to access the requested (class of) resources"@en ;
    rdfs:label "Authorization Denied Event"@en ;
    rdfs:subClassOf :AuthorizationResponse .

:AuthorizationFailed
    a owl:Class ;
    rdfs:comment "The authorization request Failed - the system could not determine if the requesting identity is authorized to access the requested (class of) resources"@en ;
    rdfs:label "Access Failed Event"@en ;
    rdfs:subClassOf :AuthorizationResponse .

:AuthorizationRequest
    a owl:Class ;
    rdfs:comment "This log entry describes a request to be granted access to particular (class of) services or resources"@en ;
    rdfs:label "Authorization Request Event"@en ;
    rdfs:subClassOf :Request .

:AuthorizationResponse
    a owl:Class ;
    rdfs:comment "This is a response to a request for Authorization - to grant an authenticated identity permission to access to (a class of) resources"@en ;
    rdfs:label "Authorization Response"@en ;
    rdfs:subClassOf :Response .

:AuthorizationSuccessful
    a owl:Class ;
    rdfs:comment "The authorization request Succeeded - the requesting identity is now authorized to access the requested (class of) resources"@en ;
    rdfs:label "Authorization Succeeded Event"@en ;
    rdfs:subClassOf :AuthorizationResponse .

:Configuration
    a owl:Class ;
    rdfs:comment "This event indicates that a change is being made in some aspect of a system's operational configuration"@en ;
    rdfs:label "Configuration Event"@en ;
    rdfs:subClassOf :LogEntry .

:ConfigurationDenied
    a owl:Class ;
    rdfs:comment "An attempt to change the configuration of this system was made, but was rejected"@en ;
    rdfs:label "Configuration Denied"@en ;
    rdfs:subClassOf :Configuration .

:ConfigurationFailed
    a owl:Class ;
    rdfs:comment "An attempt to change the configuration of this system was made, but did not complete successfully"@en ;
    rdfs:label "Configuration Failed"@en ;
    rdfs:subClassOf :Configuration .

:ConfigurationSuccessful
    a owl:Class ;
    rdfs:comment "The configuration of this system was successfully changed"@en ;
    rdfs:label "Configuration Succeeded"@en ;
    rdfs:subClassOf :Configuration .

:Critical
    a owl:Class ;
    rdfs:comment "Critical errors indicate a non-recoverable state of an operation - if other functions are dependent on this operation, they too will fail."@en ;
    rdfs:label "Non-Recoverable Error"@en ;
    rdfs:subClassOf :Error .

:Emergency
    a owl:Class ;
    rdfs:comment "Emergency errors indicate the failure of the entire subsystem"@en ;
    rdfs:label "Halting Error"@en ;
    rdfs:subClassOf :Error .

:Error
    a owl:Class ;
    rdfs:comment "This log entry describes an error in a system, encountered during runtime"@en ;
    rdfs:label "Error Event"@en ;
    rdfs:subClassOf :LogEntry .

:EventLog
    a owl:Class ;
    rdfs:comment "Microsoft's Windows EventLog format log, using semi-structured data"@en ;
    rdfs:label "Windows EventLog format log"@en ;
    rdfs:subClassOf :Log .

:Log
    a owl:Class ;
    rdfs:comment "a collection of event records ordered by time"@en ;
    rdfs:label "Log"@en ;
    rdfs:subClassOf mere:Composite, owl:Thing .

:LogEntry
    a owl:Class ;
    rdfs:comment "An event within a log source"@en ;
    rdfs:label "Log Entry"@en ;
    rdfs:subClassOf event:Event .

:Operation
    a owl:Class ;
    rdfs:comment "a software-specific operation event. These will vary greatly depending upon the purpose of the software the event is recorded from."@en ;
    rdfs:label "Operation Event"@en ;
    rdfs:subClassOf :LogEntry .

:OperationDenied
    a owl:Class ;
    rdfs:comment "The software-specific operation described here was specifically denied to be allowed to complete."@en ;
    rdfs:label "Operation Denied Event"@en ;
    rdfs:subClassOf :LogEntry .

:OperationFailed
    a owl:Class ;
    rdfs:comment "The software-specific operation described here failed to complete."@en ;
    rdfs:label "Operation Failed Event"@en ;
    rdfs:subClassOf :Operation .

:OperationSuccess
    a owl:Class ;
    rdfs:comment "The software-specific operation described here completed successfully."@en ;
    rdfs:label "Operation Succeeded Event"@en ;
    rdfs:subClassOf :LogEntry .

:RebootEvent
    a owl:Class ;
    rdfs:comment "The system was rebooted or restarted at this time"@en ;
    rdfs:label "Reboot Event"@en ;
    rdfs:subClassOf event:Event .

:Request
    a owl:Class ;
    rdfs:comment "This log entry describes a request for service"@en ;
    rdfs:label "Request Event"@en ;
    rdfs:subClassOf :LogEntry .

:Response
    a owl:Class ;
    rdfs:comment "This log entry describes a response to a request for service"@en ;
    rdfs:label "Response Event"@en ;
    rdfs:subClassOf :LogEntry .

:Session
    a owl:Class ;
    rdfs:comment "This log event tracks a specific sequence of activity (usually of an interactive nature) from a particular agent (a user, host or other client)."@en ;
    rdfs:label "Activity Session"@en ;
    rdfs:subClassOf :LogEntry .

:SessionClose
    a owl:Class ;
    rdfs:comment "The session has ended. Typically this indicates any further access will require re-authentication."@en ;
    rdfs:label "Session Closed Event"@en ;
    rdfs:subClassOf :Session .

:SessionOpen
    a owl:Class ;
    rdfs:comment "A session has been opened. Operations and access from this point on will typically require no further authentication, but authorization events may still occur."@en ;
    rdfs:label "Session Opened"@en ;
    rdfs:subClassOf :Session .

:ShutdownEvent
    a owl:Class ;
    rdfs:comment "The system was shut down at this time"@en ;
    rdfs:label "Shutdown Event"@en ;
    rdfs:subClassOf event:Event .

:SuccessfulAuthentication
    a owl:Class ;
    rdfs:comment "The authentication request succeeded and the requester is now successfully identified with the requested identity"@en ;
    rdfs:label "Authentication Succeeded Event"@en ;
    rdfs:subClassOf :AuthenticationResponse .

:Syslog
    a owl:Class ;
    rdfs:comment "the classic text-only log format, typically with a single line per log entry (although modern formats do support multiline formatting)"@en ;
    rdfs:label "Syslog format Log"@en ;
    rdfs:subClassOf :Log .

:Warning
    a owl:Class ;
    rdfs:comment "warning errors indicate a recoverable error. they will typically be followed by further attempts at the operation they reference."@en ;
    rdfs:label "Recoverable Warning Error"@en ;
    rdfs:subClassOf :Error .

:fromControl
    a owl:FunctionalProperty, owl:ObjectProperty ;
    rdfs:comment "This log contains records from a Security Control"@en ;
    rdfs:domain :Log ;
    rdfs:label "contains alert from Control"@en ;
    rdfs:range controls:Control .

:fromHost
    tapio:signaturePriority 1 ;
    a owl:FunctionalProperty, owl:ObjectProperty ;
    rdfs:comment "The source of this log or event - the viewpoint from which these events were generated from"@en ;
    rdfs:domain :Log ;
    rdfs:label "describes events on this host"@en ;
    rdfs:range host:Host, ipnet:Address .

:fromLog
    a owl:FunctionalProperty, owl:ObjectProperty ;
    rdfs:comment "The log this entry was extracted from"@en ;
    rdfs:domain :LogEntry ;
    rdfs:label "is recorded in log"@en ;
    rdfs:range :Log ;
    rdfs:subPropertyOf event:factor, mere:partOf ;
    owl:inverseOf :hasEntry .

:fromPackage
    a owl:FunctionalProperty, owl:ObjectProperty ;
    rdfs:comment "the software package this log records events from"@en ;
    rdfs:domain :Log ;
    rdfs:label "from software package"@en ;
    rdfs:range software:Package .

:fromProcess
    a owl:ObjectProperty ;
    rdfs:comment "the individual process this log records events from"@en ;
    rdfs:domain :Log ;
    rdfs:label "was generated from process"@en ;
    rdfs:range process:Process .

:hasContent
    tapio:signaturePriority 2 ;
    a owl:DatatypeProperty, owl:FunctionalProperty ;
    rdfs:comment "The original, unprocessed content of this log entry."@en ;
    rdfs:domain :LogEntry ;
    rdfs:label "original log content"@en ;
    rdfs:range :logContent ;
    rdfs:subPropertyOf event:factor .

:hasEntry
    a owl:ObjectProperty ;
    rdfs:comment "An individual, timestamped event recorded within this log"@en ;
    rdfs:domain :Log ;
    rdfs:label "has entry"@en ;
    rdfs:range :LogEntry ;
    rdfs:subPropertyOf event:factor_of, mere:hasPart ;
    owl:inverseOf :fromLog .

:isActionFromControl
    a owl:FunctionalProperty, owl:ObjectProperty ;
    rdfs:comment "This log entry is an action from a security control"@en ;
    rdfs:domain :LogEntry ;
    rdfs:label "is an action from control"@en ;
    rdfs:range host:Host ;
    rdfs:subPropertyOf event:factor, :FromControl .

:isAlertfromControl
    a owl:FunctionalProperty, owl:ObjectProperty ;
    rdfs:comment "This log entry is an alert from a security Control"@en ;
    rdfs:domain :LogEntry ;
    rdfs:label "is an alert from control"@en ;
    rdfs:range controls:Alert ;
    rdfs:subPropertyOf event:factor, :FromControl .

:logContent
    a rdfs:Datatype ;
    rdfs:comment "The raw content of a log entry, taken directly from the log source itself."@en ;
    rdfs:domain :Log ;
    rdfs:label "Log Entry Content"@en ;
    rdfs:range xsd:string .

:logLocation
    a owl:ObjectProperty ;
    rdfs:comment "The canonical location this log can be accessed from"@en ;
    rdfs:domain :Log ;
    rdfs:label "the location of this Log"@en ;
    rdfs:range filesystem:Directory, filesystem:FileName, host:Host, uri:Uri .

:referencesURI
    a owl:ObjectProperty ;
    rdfs:comment "This log entry contains a discrete URI"@en ;
    rdfs:domain :LogEntry ;
    rdfs:label "contains a URI"@en ;
    rdfs:range uri:Uri ;
    rdfs:subPropertyOf event:factor .

:requester
    a owl:FunctionalProperty, owl:ObjectProperty ;
    rdfs:comment "The entity making the request described in this log entry"@en ;
    rdfs:domain :Request ;
    rdfs:label "the source of the request"@en ;
    rdfs:range host:Host, ipnet:Address, process:Process, user:UserAccount ;
    rdfs:subPropertyOf event:agent .

:responder
    a owl:FunctionalProperty, owl:ObjectProperty ;
    rdfs:comment "The entity making the response to a request described in this log entry"@en ;
    rdfs:domain :Response ;
    rdfs:label "the target of the request"@en ;
    rdfs:range host:Host, ipnet:Address, process:Process ;
    rdfs:subPropertyOf event:factor .

